examples/enumSTProofs.v
@@ -4,33 +4,180 @@ From QuickChick Require Import QuickChick Tactics TacticsUtil Instances Classes
 Require Import String. Open Scope string.
 Require Import List micromega.Lia.
 
+Import ListNotations.
+From mathcomp Require Import ssreflect ssrfun ssrbool ssrnat eqtype seq.
 
 From Ltac2 Require Import Ltac2.
-
-Import ListNotations.
-Import QcDefaultNotation. Open Scope qc_scope.
-From mathcomp Require Import ssreflect ssrfun ssrbool ssrnat eqtype seq.
 
 Require Import enumProofs. (* TODO change *)
 
 Set Bullet Behavior "Strict Subproofs".
 
-
-(* Inductive mylist (A : Type) : Type := *)
-(*     mynil : mylist A | mycons : A -> mylist A -> mylist A. *)
-
-(* Derive EnumSized for mylist. *)
-
-Inductive In' : nat -> list nat -> Prop :=
+Inductive In' {A} : A -> list A -> Prop :=
 | In_hd :
     forall x l, In' x (cons x l)
 | In_tl :
     forall x y l, In' x l -> In' x (cons y l).
 
-(* (* XXX BUG *) *)
+
 Derive DecOpt for (In' a l).
+
+Instance DecOptIn'_listSizeMonotonic A {_ : Enum A} {_ : Dec_Eq A}
+         (x : A) (l : list A) : DecOptSizeMonotonic (In' x l).
+Proof. derive_mon (). Qed.
+
+Instance DecOptIn'_list_sound A {_ : Enum A} {_ : Dec_Eq A} (x : A) (l : list A) :
+  DecOptSoundPos (In' x l).
+Proof. derive_sound (). Qed.
+
+Instance DecOptIn'_list_complete A {_ : Enum A} {_ : Dec_Eq A} (x : A) (l : list A) :
+  DecOptCompletePos (In' x l).
+Proof. derive_complete (). Qed.
+
 Derive ArbitrarySizedSuchThat for (fun x => In' x l).
 Derive EnumSizedSuchThat for (fun x => In' x l).
+
+
+
+Ltac2 rec enumST_sized_mon (ih : ident) :=
+  first
+    [ (* ret *)
+      match! goal with
+      | [ |- ?s \subset ?s ] => now eapply subset_refl
+      end
+    | (* dec matching *)
+      match! goal with
+      | [ |- semProdSizeOpt (match @decOpt ?p ?i ?s1 with _ => _ end) _ \subset
+             semProdSizeOpt (match decOpt ?s2 with _ => _ end) _ ] =>
+        let hdec := Fresh.in_goal (id_of_string "Hdec") in 
+        destruct (@decOpt $p $i $s1) eqn:$hdec >
+        [ ((erewrite (@CheckerProofs.mon $p $i _ $s1 $s2) > [ | | eassumption ]) > [ enumST_sized_mon ih | ssromega ])
+        | rewrite (@semReturnSizeOpt_None E _ ProducerSemanticsEnum); now eapply sub0set ]
+      end
+     | (* input matching *) 
+      match! goal with
+      | [ |- semProdSizeOpt (match ?p with _ => _ end) _ \subset _ ] =>
+        destruct $p; enumST_sized_mon ih
+      end
+    | (* bindOpt *)
+      eapply (@semBindOptSizeOpt_subset_compat E _ ProducerSemanticsEnum) >
+      [ first
+          [ now eapply subset_refl (* for calls to enum *)
+          | let ih' := Control.hyp ih in (* for recursive calls *)
+            eapply $ih'; now ssromega ]
+      | let x := Fresh.in_goal (id_of_string "x") in
+        intros $x; enumST_sized_mon ih
+      ]
+    | (* bind *)
+      eapply (@semBindSizeOpt_subset_compat E _ ProducerSemanticsEnum) >
+      [ now eapply subset_refl 
+      | let x := Fresh.in_goal (id_of_string "x") in
+        intros $x; enumST_sized_mon ih
+      ]
+    | ()
+    ].
+
+Ltac2 rec find_enumST (ih : ident) :=
+  first
+    [ now eapply incl_bigcup_list_nil
+    | eapply incl_bigcup_compat_list > [ (now enumST_sized_mon ih)  | find_enumST ih ]
+    | eapply incl_bigcup_list_tl; find_enumST ih
+    ].
+
+Ltac2 base_case_st_size_mon (s2 : constr) :=
+  destruct $s2 > 
+  [ first [ now eapply subset_refl | rewrite !enumerate_correct_size_opt; find_enumST @dummy ]
+  | rewrite !enumerate_correct_size_opt; find_enumST @dummy ]. 
+
+Ltac2 ind_case_st_sized_mon (s2 : constr) (ih : ident) :=
+  destruct $s2 > 
+  [ now ssromega |  rewrite !enumerate_correct_size_opt; (* find_enumST ih *) () ]. 
+
+Ltac2 derive_enumST_SizedMonotonic (_ : unit) :=
+  match! goal with
+  | [ |- SizedMonotonicOpt (@enumSizeST ?typ ?pred ?inst) ] =>
+    assert (Henum := @enumerate_correct_size $typ);
+      
+    let s := Fresh.in_goal (id_of_string "s") in
+    let s1 := Fresh.in_goal (id_of_string "s1") in
+    let s2 := Fresh.in_goal (id_of_string "s2") in
+    let s1i := Fresh.in_goal (id_of_string "s1i") in
+    let s2i := Fresh.in_goal (id_of_string "s2i") in
+    let hleq := Fresh.in_goal (id_of_string "Hleq") in
+    let hleqi := Fresh.in_goal (id_of_string "Hleqi") in
+    let ihs1 := Fresh.in_goal (id_of_string "ihs1") in
+    intros $s $s1 $s2 $hleq; simpl_enumSizeST ();
+      let hleq' := Control.hyp hleq in
+      let s1' := Control.hyp s1 in
+      let s2' := Control.hyp s2 in
+      assert ($hleqi := $hleq');
+      revert $hleqi $hleq;
+      generalize $s2' at 1 3; generalize $s1' at 1 3; revert $s $s2; revert_params inst;
+        (induction $s1' as [| $s1 $ihs1 ]; intro_params inst; intros $s $s2 $s1i $s2i $hleqi $hleq) >
+        [ base_case_st_size_mon s2' | ind_case_st_sized_mon s2' ihs1  ]
+  end.
+
+
+
+
+
+
+Instance EnumSizedSuchThatIn'_SizedMonotonic A {_ : Enum A} l :
+  SizedMonotonicOpt (@enumSizeST _ _ (EnumSizedSuchThatIn' l)).
+Proof. derive_enumST_SizedMonotonic ().
+
+       eapply incl_bigcup_compat_list.
+       now enumST_sized_mon @ihs1.
+
+       eapply incl_bigcup_compat_list.
+
+
+Ltac2 rec enumST_sized_mon (ih : ident) :=
+  first
+    [ (* ret *)
+      match! goal with
+      | [ |- ?s \subset ?s ] => now eapply subset_refl
+      end
+    | (* dec matching *)
+      match! goal with
+      | [ |- semProdSizeOpt (match @decOpt ?p ?i ?s1 with _ => _ end) _ \subset
+             semProdSizeOpt (match decOpt ?s2 with _ => _ end) _ ] =>
+        let hdec := Fresh.in_goal (id_of_string "Hdec") in 
+        destruct (@decOpt $p $i $s1) eqn:$hdec >
+        [ ((erewrite (@CheckerProofs.mon $p $i _ $s1 $s2) > [ | | eassumption ]) > [ (* enumST_sized_mon ih *) | ssromega ])
+        | rewrite (@semReturnSizeOpt_None E _ ProducerSemanticsEnum); now eapply sub0set ]
+      end
+     | (* input matching *) 
+      match! goal with
+      | [ |- semProdSizeOpt (match ?p with _ => _ end) _ \subset _ ] =>
+        destruct $p; (* enumST_sized_mon ih *) ()
+      end
+    | (* bindOpt *)
+      eapply (@semBindOptSizeOpt_subset_compat E _ ProducerSemanticsEnum) >
+      [ first
+          [ now eapply subset_refl (* for calls to enum *)
+          | let ih' := Control.hyp ih in (* for recursive calls *)
+            eapply $ih'; now ssromega ]
+      | let x := Fresh.in_goal (id_of_string "x") in
+        intros $x; (* enumST_sized_mon ih *) ()
+      ]
+    | (* bind *)
+      eapply (@semBindSizeOpt_subset_compat E _ ProducerSemanticsEnum) >
+      [ now eapply subset_refl 
+      | let x := Fresh.in_goal (id_of_string "x") in
+        intros $x; enumST_sized_mon ih
+      ]
+    | ()
+    ].
+
+
+
+       now enumST_sized_mon @ihs1.
+
+Qed.
+
+
+
 
 Inductive ltest : list nat -> nat -> Prop :=
   | ltestnil :
